Prove tick removal function pres. semantics for BVL
The plan is to compose this with inline so that we have
an inline function that doesn't add Tick (required for
Oskar's bvi_tailrec optimisation to be triggered).

compiler/backend/proofs/bvl_inlineProofScript.sml
@@ -377,4 +377,507 @@ val MAP_FST_compile_prog = Q.store_thm("MAP_FST_compile_prog",
   `MAP FST (bvl_inline$compile_prog limit prog) = MAP FST prog`,
   fs [bvl_inlineTheory.compile_prog_def] \\ rw [MAP_FST_inline_all]);
 
+(* removal of ticks *)
+
+val remove_ticks_def = tDefine "remove_ticks" `
+  (remove_ticks [] = []) /\
+  (remove_ticks (x::y::xs) =
+     HD (remove_ticks [x]) :: remove_ticks (y::xs)) /\
+  (remove_ticks [Var v] = [Var v]) /\
+  (remove_ticks [If x1 x2 x3] =
+     [If (HD (remove_ticks [x1]))
+         (HD (remove_ticks [x2]))
+         (HD (remove_ticks [x3]))]) /\
+  (remove_ticks [Let xs x2] =
+     [Let (remove_ticks xs) (HD (remove_ticks [x2]))]) /\
+  (remove_ticks [Raise x1] =
+     [Raise (HD (remove_ticks [x1]))]) /\
+  (remove_ticks [Handle x1 x2] =
+     [Handle (HD (remove_ticks [x1]))
+             (HD (remove_ticks [x2]))]) /\
+  (remove_ticks [Op op xs] =
+     [Op op (remove_ticks xs)]) /\
+  (remove_ticks [Tick x] = remove_ticks [x]) /\
+  (remove_ticks [Call ticks dest xs] =
+     [Call 0 dest (remove_ticks xs)])`
+  (WF_REL_TAC `measure exp1_size`);
+
+val LENGTH_remove_ticks = store_thm("LENGTH_remove_ticks[simp]",
+  ``!xs. LENGTH (remove_ticks xs) = LENGTH xs``,
+  recInduct (theorem "remove_ticks_ind") \\ fs [remove_ticks_def]);
+
+val remove_ticks_SING = store_thm("remove_ticks_SING[simp]",
+  ``[HD (remove_ticks [r])] = remove_ticks [r]``,
+  qsuff_tac `?a. remove_ticks [r] = [a]` \\ rw[] \\ fs []
+  \\ `LENGTH (remove_ticks [r]) = LENGTH [r]` by fs [LENGTH_remove_ticks]
+  \\ Cases_on `remove_ticks [r]` \\ fs []);
+
+val state_rel_def = Define `
+  state_rel (s:'ffi bvlSem$state) (t:'ffi bvlSem$state) <=>
+    t = s with code := map (I ## (\x. HD (remove_ticks [x]))) s.code`
+
+val do_app_lemma = prove(
+  ``state_rel t' r ==>
+    case do_app op (REVERSE a) r of
+    | Rerr err => do_app op (REVERSE a) t' = Rerr err
+    | Rval (v,r2) => ?t2. state_rel t2 r2 /\ do_app op (REVERSE a) t' = Rval (v,t2)``,
+  strip_tac \\ Cases_on `do_app op (REVERSE a) t'`
+  THEN1
+   (PairCases_on `a'`
+    \\ drule (GEN_ALL bvlPropsTheory.do_app_with_code)
+    \\ disch_then (qspec_then `r.code` mp_tac)
+    \\ fs [state_rel_def,domain_map]
+    \\ rw [] \\ fs [state_component_equality]
+    \\ imp_res_tac do_app_const \\ fs [])
+  \\ drule (GEN_ALL bvlPropsTheory.do_app_with_code_err)
+  \\ disch_then (qspec_then `r.code` mp_tac)
+  \\ fs [state_rel_def,domain_map]);
+
+val evaluate_remove_ticks = Q.store_thm("evaluate_remove_ticks",
+  `!k xs env s (t:'ffi bvlSem$state) res s'.
+      state_rel t s /\ s.clock = k /\
+      evaluate (remove_ticks xs,env,s) = (res,s') ==>
+      ?ck t'. evaluate (xs,env,t with clock := t.clock + ck) = (res,t') /\
+              state_rel t' s'`,
+  strip_tac \\ completeInduct_on `k` \\ fs [PULL_FORALL,AND_IMP_INTRO]
+  \\ recInduct (theorem "remove_ticks_ind") \\ rw []
+  THEN1 (* NIL *)
+   (fs [evaluate_def,remove_ticks_def] \\ rveq
+    \\ qexists_tac `0` \\ fs [state_rel_def,state_component_equality])
+  THEN1 (* CONS *)
+   (fs [evaluate_def,remove_ticks_def]
+    \\ pop_assum mp_tac \\ simp [Once evaluate_CONS]
+    \\ TOP_CASE_TAC
+    \\ qpat_x_assum `!x. _` mp_tac
+    \\ first_x_assum drule \\ fs []
+    \\ disch_then drule \\ strip_tac
+    \\ reverse (Cases_on `q`) \\ fs []
+    THEN1 (rw [] \\ fs [] \\ qexists_tac `ck` \\ fs [])
+    \\ strip_tac
+    \\ `∀env s' (t:'ffi bvlSem$state) res s''.
+         state_rel t s' ∧ s'.clock <= s.clock ∧
+         evaluate (remove_ticks (y::xs),env,s') = (res,s'') ⇒
+         ∃ck t'.
+           evaluate (y::xs,env,t with clock := ck + t.clock) = (res,t') ∧
+           state_rel t' s''` by metis_tac [LESS_OR_EQ]
+    \\ pop_assum drule
+    \\ imp_res_tac evaluate_clock \\ fs []
+    \\ TOP_CASE_TAC \\ disch_then drule \\ strip_tac
+    \\ rw [] \\ qexists_tac `ck+ck'`
+    \\ qpat_x_assum `evaluate ([x],_) = _` assume_tac
+    \\ drule evaluate_add_clock \\ fs [inc_clock_def]
+    \\ disch_then kall_tac
+    \\ CASE_TAC \\ fs [])
+  THEN1 (* Var *)
+   (fs [evaluate_def,remove_ticks_def]
+    \\ CASE_TAC \\ fs [] \\ rveq
+    \\ qexists_tac `0` \\ fs [state_rel_def,state_component_equality])
+  THEN1 (* If *)
+   (fs [evaluate_def,remove_ticks_def]
+    \\ pop_assum mp_tac \\ TOP_CASE_TAC
+    \\ qpat_x_assum `!x. _` mp_tac
+    \\ qpat_x_assum `!x. _` mp_tac
+    \\ first_x_assum drule \\ fs []
+    \\ disch_then drule \\ strip_tac
+    \\ reverse (Cases_on `q`) \\ fs []
+    THEN1 (rw [] \\ fs [] \\ qexists_tac `ck` \\ fs [])
+    \\ TOP_CASE_TAC THEN1
+     (disch_then assume_tac \\ disch_then kall_tac \\ strip_tac
+      \\ `∀env s' (t:'ffi bvlSem$state) res s''.
+           state_rel t s' ∧ s'.clock <= s.clock ∧
+           evaluate (remove_ticks [x2],env,s') = (res,s'') ⇒
+           ∃ck t'.
+             evaluate ([x2],env,t with clock := ck + t.clock) = (res,t') ∧
+             state_rel t' s''` by metis_tac [LESS_OR_EQ]
+      \\ first_x_assum drule
+      \\ imp_res_tac evaluate_clock \\ fs []
+      \\ disch_then drule \\ strip_tac
+      \\ rw [] \\ qexists_tac `ck+ck'`
+      \\ qpat_x_assum `evaluate ([x1],_) = _` assume_tac
+      \\ drule evaluate_add_clock \\ fs [inc_clock_def]
+      \\ disch_then kall_tac)
+    \\ TOP_CASE_TAC THEN1
+     (disch_then kall_tac \\ disch_then assume_tac \\ strip_tac
+      \\ `∀env s' (t:'ffi bvlSem$state) res s''.
+           state_rel t s' ∧ s'.clock <= s.clock ∧
+           evaluate (remove_ticks [x3],env,s') = (res,s'') ⇒
+           ∃ck t'.
+             evaluate ([x3],env,t with clock := ck + t.clock) = (res,t') ∧
+             state_rel t' s''` by metis_tac [LESS_OR_EQ]
+      \\ first_x_assum drule
+      \\ imp_res_tac evaluate_clock \\ fs []
+      \\ disch_then drule \\ strip_tac
+      \\ rw [] \\ qexists_tac `ck+ck'`
+      \\ qpat_x_assum `evaluate ([x1],_) = _` assume_tac
+      \\ drule evaluate_add_clock \\ fs [inc_clock_def]
+      \\ disch_then kall_tac)
+    \\ rw [] \\ qexists_tac `ck` \\ fs [])
+  THEN1 (* Let *)
+   (fs [evaluate_def,remove_ticks_def]
+    \\ pop_assum mp_tac \\ TOP_CASE_TAC
+    \\ qpat_x_assum `!x. _` mp_tac
+    \\ first_x_assum drule \\ fs []
+    \\ disch_then drule \\ strip_tac
+    \\ reverse (Cases_on `q`) \\ fs []
+    THEN1 (rw [] \\ fs [] \\ qexists_tac `ck` \\ fs [])
+    \\ strip_tac
+    \\ `∀env s' (t:'ffi bvlSem$state) res s''.
+           state_rel t s' ∧ s'.clock <= s.clock ∧
+           evaluate (remove_ticks [x2],env,s') = (res,s'') ⇒
+           ∃ck t'.
+             evaluate ([x2],env,t with clock := ck + t.clock) = (res,t') ∧
+             state_rel t' s''` by metis_tac [LESS_OR_EQ]
+    \\ first_x_assum drule
+    \\ imp_res_tac evaluate_clock \\ fs []
+    \\ rpt strip_tac \\ first_x_assum drule
+    \\ rw [] \\ qexists_tac `ck+ck'`
+    \\ qpat_x_assum `evaluate (xs,_) = _` assume_tac
+    \\ drule evaluate_add_clock \\ fs [inc_clock_def])
+  THEN1 (* Raise *)
+   (fs [evaluate_def,remove_ticks_def]
+    \\ pop_assum mp_tac \\ TOP_CASE_TAC
+    \\ first_x_assum drule \\ fs []
+    \\ disch_then drule \\ strip_tac
+    \\ reverse (Cases_on `q`) \\ fs []
+    \\ rw [] \\ fs [] \\ qexists_tac `ck` \\ fs [])
+  THEN1 (* Handle *)
+   (fs [evaluate_def,remove_ticks_def]
+    \\ pop_assum mp_tac \\ TOP_CASE_TAC
+    \\ qpat_x_assum `!x. _` mp_tac
+    \\ first_x_assum drule \\ fs []
+    \\ disch_then drule \\ strip_tac
+    \\ Cases_on `q` \\ fs []
+    THEN1 (rw [] \\ fs [] \\ qexists_tac `ck` \\ fs [])
+    \\ reverse (Cases_on `e`) \\ fs []
+    THEN1 (rw [] \\ fs [] \\ qexists_tac `ck` \\ fs [])
+    \\ rpt strip_tac
+    \\ `∀env s' (t:'ffi bvlSem$state) res s''.
+           state_rel t s' ∧ s'.clock <= s.clock ∧
+           evaluate (remove_ticks [x2],env,s') = (res,s'') ⇒
+           ∃ck t'.
+             evaluate ([x2],env,t with clock := ck + t.clock) = (res,t') ∧
+             state_rel t' s''` by metis_tac [LESS_OR_EQ]
+    \\ first_x_assum drule
+    \\ imp_res_tac evaluate_clock \\ fs []
+    \\ rpt strip_tac \\ first_x_assum drule
+    \\ rw [] \\ qexists_tac `ck+ck'`
+    \\ qpat_x_assum `evaluate ([x1],_) = _` assume_tac
+    \\ drule evaluate_add_clock \\ fs [inc_clock_def])
+  THEN1 (* Op *)
+   (fs [remove_ticks_def,evaluate_def]
+    \\ FULL_CASE_TAC \\ fs []
+    \\ first_x_assum drule \\ fs []
+    \\ disch_then drule \\ strip_tac
+    \\ qexists_tac `ck` \\ fs []
+    \\ reverse (Cases_on `q`) \\ fs [] \\ rveq \\ fs []
+    \\ drule do_app_lemma \\ every_case_tac \\ fs []
+    \\ rveq \\ fs [])
+  THEN1 (* Tick *)
+   (fs [remove_ticks_def]
+    \\ first_x_assum drule \\ fs []
+    \\ disch_then drule \\ strip_tac
+    \\ fs [bvlSemTheory.evaluate_def]
+    \\ qexists_tac `ck + 1` \\ fs [dec_clock_def])
+  (* Call *)
+  \\ fs [remove_ticks_def]
+  \\ fs [bvlSemTheory.evaluate_def]
+  \\ FULL_CASE_TAC \\ fs []
+  \\ reverse (Cases_on `q`) \\ fs [] \\ rveq
+  THEN1
+   (first_x_assum drule \\ fs []
+    \\ disch_then drule \\ strip_tac
+    \\ qexists_tac `ck` \\ fs [])
+  \\ pop_assum mp_tac
+  \\ TOP_CASE_TAC \\ fs [] \\ rpt strip_tac \\ rveq \\ fs []
+  THEN1
+   (first_x_assum drule \\ fs []
+    \\ disch_then drule \\ strip_tac
+    \\ qexists_tac `ck` \\ fs []
+    \\ qsuff_tac `find_code dest a t'.code = NONE` \\ fs []
+    \\ Cases_on `dest` \\ fs [find_code_def]
+    \\ every_case_tac \\ fs [state_rel_def]
+    \\ rveq \\ fs [lookup_map]
+    \\ PairCases_on `z` \\ fs [])
+  \\ PairCases_on `x` \\ fs []
+  \\ pop_assum mp_tac
+  \\ IF_CASES_TAC \\ rw []
+  THEN1
+   (first_x_assum drule \\ fs []
+    \\ disch_then drule \\ strip_tac
+    \\ qexists_tac `ck` \\ fs []
+    \\ qsuff_tac `?x1 x2. find_code dest a t'.code = SOME (x1,x2)`
+    THEN1 (strip_tac \\ fs [] \\ fs [state_rel_def])
+    \\ fs [state_rel_def] \\ rveq \\ fs []
+    \\ Cases_on `dest` \\ fs [find_code_def]
+    \\ every_case_tac \\ fs [] \\ rveq \\ fs [lookup_map] \\ fs []
+    \\ PairCases_on `z` \\ fs [])
+  \\ first_x_assum drule \\ fs []
+  \\ disch_then drule \\ strip_tac
+  \\ `(dec_clock 1 r).clock < s.clock` by
+        (imp_res_tac evaluate_clock  \\ fs [dec_clock_def] \\ fs [])
+  \\ first_x_assum drule
+  \\ `state_rel (dec_clock 1 t') (dec_clock 1 r)` by fs [state_rel_def]
+  \\ disch_then drule
+  \\ `?a2. find_code dest a t'.code = SOME (x0,a2) /\
+           [x1] = remove_ticks [a2]` by
+   (Cases_on `dest` \\ fs [state_rel_def,find_code_def] \\ rveq \\ fs []
+    \\ every_case_tac \\ fs [lookup_map] \\ rveq \\ fs []
+    \\ rveq \\ fs [])
+  \\ fs [] \\ disch_then drule \\ strip_tac
+  \\ ntac 2 (pop_assum mp_tac)
+  \\ drule evaluate_add_clock \\ fs [inc_clock_def]
+  \\ disch_then (qspec_then `ticks+ck'` assume_tac)
+  \\ rw [] \\ qexists_tac `ticks + ck+ck'` \\ fs [dec_clock_def]
+  \\ qsuff_tac `t'.clock <> 0` \\ rpt strip_tac \\ fs []
+  \\ fs [state_rel_def]);
+
+val evaluate_remove_ticks_thm =
+  evaluate_remove_ticks
+  |> SIMP_RULE std_ss []
+  |> Q.SPEC `[Call 0 (SOME start) []]`
+  |> SIMP_RULE std_ss [remove_ticks_def];
+
+val evaluate_compile_prog = Q.store_thm ("evaluate_compile_prog",
+  `evaluate ([Call 0 (SOME start) []], [],
+             initial_state ffi0 (map
+                (I ## (λx. HD (remove_ticks [x]))) prog) k) = (r, s) ⇒
+   ∃ck (s2:'ffi bvlSem$state).
+     evaluate
+      ([Call 0 (SOME start) []], [],
+        initial_state ffi0 prog (k + ck)) = (r, s2) ∧
+     s2.ffi = s.ffi`,
+  strip_tac
+  \\ drule (ONCE_REWRITE_RULE [CONJ_COMM]
+             (REWRITE_RULE [CONJ_ASSOC] evaluate_remove_ticks_thm))
+  \\ disch_then (qspec_then `initial_state ffi0 prog k` mp_tac)
+  \\ impl_tac THEN1 fs [state_rel_def]
+  \\ strip_tac \\ fs []
+  \\ qexists_tac `ck` \\ fs [state_rel_def]);
+
+val FST_EQ_LEMMA = prove(
+  ``FST x = y <=> ?y1. x = (y,y1)``,
+  Cases_on `x` \\ fs []);
+
+val compile_prog_semantics = Q.store_thm ("compile_prog_semantics",
+  `semantics ffi (map (I ## (λx. HD (remove_ticks [x]))) prog) start =
+   semantics ffi prog start`,
+  simp [Once semantics_def]
+  \\ IF_CASES_TAC \\ fs []
+  THEN1
+   (simp [semantics_def] \\ IF_CASES_TAC \\ fs [FST_EQ_LEMMA]
+    \\ drule evaluate_compile_prog \\ metis_tac [])
+  \\ DEEP_INTRO_TAC some_intro \\ simp []
+  \\ conj_tac
+  >-
+   (gen_tac \\ strip_tac \\ rveq \\ simp []
+    \\ simp [semantics_def]
+    \\ IF_CASES_TAC \\ fs []
+    >-
+      (first_assum (subterm (fn tm => Cases_on`^(assert(has_pair_type)tm)`) o concl)
+      \\ drule evaluate_add_clock
+      \\ impl_tac >- fs []
+      \\ strip_tac
+      \\ qpat_x_assum `evaluate (_,_,_ _ (_ prog) _) = _` kall_tac
+      \\ last_assum (qspec_then `k'` mp_tac)
+      \\ (fn g => subterm (fn tm => Cases_on`^(assert(has_pair_type)tm)`) (#2 g) g )
+      \\ drule (GEN_ALL evaluate_compile_prog) \\ simp []
+      \\ strip_tac
+      \\ first_x_assum (qspec_then `ck` mp_tac)
+      \\ simp [inc_clock_def]
+      \\ rw[] \\ fs [])
+    \\ DEEP_INTRO_TAC some_intro \\ simp []
+    \\ conj_tac
+    >-
+     (gen_tac \\ strip_tac \\ rveq \\ fs []
+      \\ qabbrev_tac `opts = (map (I ## (λx. HD (remove_ticks [x]))) prog)`
+      \\ qmatch_assum_abbrev_tac `bvlSem$evaluate (opts1,[],sopt1) = _`
+      \\ qmatch_assum_abbrev_tac `bvlSem$evaluate (exps1,[],st1) = (r,s)`
+      \\ qspecl_then [`opts1`,`[]`,`sopt1`] mp_tac
+           evaluate_add_to_clock_io_events_mono
+      \\ qspecl_then [`exps1`,`[]`,`st1`] mp_tac
+           evaluate_add_to_clock_io_events_mono
+      \\ simp [inc_clock_def, Abbr`sopt1`, Abbr`st1`]
+      \\ ntac 2 strip_tac
+      \\ Cases_on `s.ffi.final_event` \\ fs []
+      >-
+        (Cases_on `s'.ffi.final_event` \\ fs []
+        >-
+          (unabbrev_all_tac
+          \\ drule (GEN_ALL evaluate_compile_prog) \\ simp []
+          \\ strip_tac
+          \\ drule evaluate_add_clock
+          \\ impl_tac
+          >- (every_case_tac \\ fs [])
+          \\ rveq
+          \\ disch_then (qspec_then `k'` mp_tac) \\ simp [inc_clock_def]
+          \\ qpat_x_assum `evaluate _ = _` kall_tac
+          \\ drule evaluate_add_clock
+          \\ impl_tac
+          >- (spose_not_then strip_assume_tac \\ fs [evaluate_def])
+          \\ disch_then (qspec_then `ck+k` mp_tac) \\ simp [inc_clock_def]
+          \\ ntac 2 strip_tac \\ rveq \\ fs []
+          \\ fs [state_component_equality, state_rel_def])
+        \\ qpat_x_assum `∀extra._` mp_tac
+        \\ first_x_assum (qspec_then `k'` assume_tac)
+        \\ first_assum (subterm
+             (fn tm => Cases_on`^(assert has_pair_type tm)`) o concl)
+        \\ strip_tac \\ fs []
+        \\ unabbrev_all_tac
+        \\ drule (GEN_ALL evaluate_compile_prog)
+        \\ strip_tac
+        \\ qhdtm_x_assum `evaluate` mp_tac
+        \\ imp_res_tac evaluate_add_clock
+        \\ pop_assum mp_tac
+        \\ ntac 2 (pop_assum kall_tac)
+        \\ impl_tac
+        >- (strip_tac \\ fs [])
+        \\ disch_then (qspec_then `k'` mp_tac) \\ simp [inc_clock_def]
+        \\ first_x_assum (qspec_then `ck + k` mp_tac) \\ fs []
+        \\ ntac 3 strip_tac
+        \\ fs [state_rel_def] \\ rveq)
+      \\ qpat_x_assum `∀extra._` mp_tac
+      \\ first_x_assum (qspec_then `k'` assume_tac)
+      \\ first_assum (subterm (fn tm =>
+            Cases_on`^(assert has_pair_type tm)`) o concl)
+      \\ fs []
+      \\ unabbrev_all_tac
+      \\ strip_tac
+      \\ drule (GEN_ALL evaluate_compile_prog)
+      \\ strip_tac \\ rveq \\ fs []
+      \\ reverse (Cases_on `s'.ffi.final_event`) \\ fs [] \\ rfs []
+      >-
+        (first_x_assum (qspec_then `ck + k` mp_tac)
+        \\ fs [ADD1]
+        \\ strip_tac \\ fs [state_rel_def] \\ rfs [])
+      \\ qhdtm_x_assum `evaluate` mp_tac
+      \\ imp_res_tac evaluate_add_clock
+      \\ pop_assum kall_tac
+      \\ pop_assum mp_tac
+      \\ impl_tac
+      >- (strip_tac \\ fs [])
+      \\ disch_then (qspec_then `ck + k` mp_tac)
+      \\ simp [inc_clock_def]
+      \\ rpt strip_tac \\ rveq
+      \\ CCONTR_TAC \\ fs []
+      \\ rveq \\ fs [] \\ rfs [])
+    \\ qmatch_assum_abbrev_tac `bvlSem$evaluate (exps2,[],st2) = _`
+    \\ qspecl_then [`exps2`,`[]`,`st2`] mp_tac evaluate_add_to_clock_io_events_mono
+    \\ simp [inc_clock_def, Abbr`st2`]
+    \\ disch_then (qspec_then `0` strip_assume_tac)
+    \\ first_assum (subterm (fn tm => Cases_on`^(assert(has_pair_type)tm)`) o concl)
+    \\ unabbrev_all_tac
+    \\ drule (GEN_ALL evaluate_compile_prog)
+    \\ strip_tac
+    \\ asm_exists_tac \\ fs []
+    \\ every_case_tac \\ fs [] \\ rveq \\ fs [])
+  \\ strip_tac
+  \\ simp [semantics_def]
+  \\ IF_CASES_TAC \\ fs []
+  >-
+    (last_x_assum (qspec_then `k` assume_tac) \\ rfs []
+    \\ first_assum (qspec_then `e` assume_tac)
+    \\ fs [] \\ rfs []
+    \\ qmatch_assum_abbrev_tac `FST q ≠ _`
+    \\ Cases_on `q` \\ fs [markerTheory.Abbrev_def]
+    \\ pop_assum (assume_tac o SYM)
+    \\ drule (GEN_ALL evaluate_compile_prog)
+    \\ simp []
+    \\ spose_not_then strip_assume_tac
+    \\ qmatch_assum_abbrev_tac `FST q = _`
+    \\ Cases_on `q` \\ fs [markerTheory.Abbrev_def]
+    \\ pop_assum (assume_tac o SYM)
+    \\ imp_res_tac evaluate_add_clock \\ rfs []
+    \\ first_x_assum (qspec_then `ck` mp_tac)
+    \\ simp [inc_clock_def])
+  \\ DEEP_INTRO_TAC some_intro \\ simp []
+  \\ conj_tac
+  >-
+    (spose_not_then assume_tac \\ rw []
+    \\ fsrw_tac [QUANT_INST_ss[pair_default_qp]] []
+    \\ last_assum (qspec_then `k` mp_tac)
+    \\ (fn g => subterm (fn tm => Cases_on`^(assert (can dest_prod o type_of) tm)` g) (#2 g))
+    \\ strip_tac
+    \\ drule (GEN_ALL evaluate_compile_prog)
+    \\ strip_tac
+    \\ qmatch_assum_rename_tac `evaluate (_,[],_ k) = (_,rr)`
+    \\ reverse (Cases_on `rr.ffi.final_event`)
+    >-
+      (first_x_assum
+        (qspecl_then
+          [`k`, `FFI_outcome(THE rr.ffi.final_event)`] mp_tac)
+      \\ simp [])
+    \\ qpat_x_assum `∀x y. ¬z` mp_tac \\ simp []
+    \\ qexists_tac `k` \\ simp []
+    \\ reverse (Cases_on `s.ffi.final_event`) \\ fs []
+    >-
+      (qhdtm_x_assum `evaluate` mp_tac
+      \\ qmatch_assum_abbrev_tac `bvlSem$evaluate (opts1,[],os1) = (r,_)`
+      \\ qspecl_then [`opts1`,`[]`,`os1`] mp_tac evaluate_add_to_clock_io_events_mono
+      \\ disch_then (qspec_then `ck` mp_tac)
+      \\ fs [ADD1, inc_clock_def, Abbr`os1`]
+      \\ rpt strip_tac \\ fs []
+      \\ fs [state_rel_def] \\ rfs [])
+    \\ qhdtm_x_assum `evaluate` mp_tac
+    \\ imp_res_tac evaluate_add_clock
+    \\ pop_assum mp_tac
+    \\ impl_tac
+    >- (strip_tac \\ fs [])
+    \\ disch_then (qspec_then `ck` mp_tac)
+    \\ simp [inc_clock_def]
+    \\ fs [ADD1]
+    \\ rpt strip_tac \\ rveq \\ fs [])
+  \\ strip_tac
+  \\ qmatch_abbrev_tac `build_lprefix_lub l1 = build_lprefix_lub l2`
+  \\ `(lprefix_chain l1 ∧ lprefix_chain l2) ∧ equiv_lprefix_chain l1 l2`
+     suffices_by metis_tac [build_lprefix_lub_thm,
+                            lprefix_lub_new_chain,
+                            unique_lprefix_lub]
+  \\ conj_asm1_tac
+  >-
+    (unabbrev_all_tac
+    \\ conj_tac
+    \\ Ho_Rewrite.ONCE_REWRITE_TAC [GSYM o_DEF]
+    \\ REWRITE_TAC [IMAGE_COMPOSE]
+    \\ match_mp_tac prefix_chain_lprefix_chain
+    \\ simp [prefix_chain_def, PULL_EXISTS]
+    \\ qx_genl_tac [`k1`,`k2`]
+    \\ qspecl_then [`k1`,`k2`] mp_tac LESS_EQ_CASES
+    \\ metis_tac [
+         LESS_EQ_EXISTS,
+         bviPropsTheory.initial_state_with_simp,
+         bvlPropsTheory.initial_state_with_simp,
+         bviPropsTheory.evaluate_add_to_clock_io_events_mono
+           |> CONV_RULE(RESORT_FORALL_CONV(sort_vars["s"]))
+           |> Q.SPEC`s with clock := k`
+           |> SIMP_RULE (srw_ss())[bviPropsTheory.inc_clock_def],
+         bvlPropsTheory.evaluate_add_to_clock_io_events_mono
+           |> CONV_RULE(RESORT_FORALL_CONV(sort_vars["s"]))
+           |> Q.SPEC`s with clock := k`
+           |> SIMP_RULE (srw_ss())[bvlPropsTheory.inc_clock_def]])
+  \\ simp [equiv_lprefix_chain_thm]
+  \\ unabbrev_all_tac \\ simp [PULL_EXISTS]
+  \\ simp [LNTH_fromList, PULL_EXISTS, GSYM FORALL_AND_THM]
+  \\ rpt gen_tac
+  \\ Cases_on `(evaluate
+         ([Call 0 (SOME start) []],[],
+          initial_state ffi
+            (map (I ## (λx. HD (remove_ticks [x]))) prog) k))`
+  \\ drule (GEN_ALL evaluate_compile_prog)
+  \\ strip_tac \\ fs []
+  \\ conj_tac \\ rw []
+  >- (qexists_tac `ck + k`
+      \\ fs [])
+  \\ qexists_tac `k` \\ fs []
+  \\ qmatch_assum_abbrev_tac `_ < (LENGTH (_ ffi1))`
+  \\ `ffi1.io_events ≼ r.ffi.io_events` by
+    (qunabbrev_tac `ffi1`
+    \\ metis_tac [
+       initial_state_with_simp, evaluate_add_to_clock_io_events_mono
+         |> CONV_RULE(RESORT_FORALL_CONV(sort_vars["s"]))
+         |> Q.SPEC`s with clock := k`
+         |> SIMP_RULE(srw_ss())[inc_clock_def],
+       SND,ADD_SYM])
+  \\ fs [IS_PREFIX_APPEND]
+  \\ simp [EL_APPEND1]);
+
 val _ = export_theory();
